@prefix rdfg: <http://www.w3.org/2004/03/trix/rdfg-1/> .
@prefix rdfs: <http://www.w3.org/2000/01/rdf-schema#> .
@prefix rdf: <http://www.w3.org/1999/02/22-rdf-syntax-ns#> .
@prefix xsd: <http://www.w3.org/2001/XMLSchema#> .
@prefix owl: <http://www.w3.org/2002/07/owl#> .
@prefix bibo: <http://purl.org/ontology/bibo/> .
@prefix dcterms: <http://purl.org/dc/terms/> .
@prefix pad: <http://purl.org/job/pad/> .
@prefix xsd: <http://www.w3.org/2001/XMLSchema#> .

pad: a owl:Ontology ;
    dcterms:title "PAD, the Platform Assertion Document Framework" ;
    dcterms:creator "Bram van den Boomen" ;
    dcterms:creator "Nees-Jan van Eck" ;
    dcterms:creator "Ludo Waltman" ;
    dcterms:creator "Serge Horbach" ;
    dcterms:creator "Tony Ross-Hellauer" ;
    dcterms:license <https://creativecommons.org/publicdomain/zero/1.0/> ;
    dcterms:date "2023-04-21" ;
    dcterms:description """
TODO: Introduction (markdown)
"""@en ;
    dcterms:abstract """
TODO: Abstract
"""@en ;
    bibo:status "Ontology Specification Draft" ;
    owl:versionInfo "0.1.0" .

pad:Assertion a rdfg:Graph ;
    rdfs:label "Assertion"@en ;
    rdfs:comment "Graph that contains statements about a platform."@en .

pad:PubInfo a rdfg:Graph ;
    rdfs:label "PADInfo"@en ;
    rdfs:comment "Graph that contains statements about a Platform Assertion Document."@en .

pad:PAD a rdfs:Class ;
    rdfs:label "Platform Assertion Document"@en ;
    rdfs:comment "A Platform Assertion Document, providing machine readable, tracable way to codify information about scholarly communication platforms."@en .

pad:Provenance a rdfg:Graph ;
    rdfs:label "Provenance"@en ;
    rdfs:comment "Graph that contains statements about an Assertion."@en .

pad:hasAssertion a owl:FunctionalProperty ;
    rdfs:domain pad:PAD ;
    rdfs:range pad:Assertion ;
    rdfs:label "has Assertion"@en ;
    rdfs:comment "The property relating a Platform Assertion Document to an Assertion."@en .

pad:hasPubInfo a owl:FunctionalProperty ;
    rdfs:domain pad:PAD ;
    rdfs:range pad:DocInfo ;
    rdfs:label ""@en ;
    rdfs:comment "The property relating a Platform Assertion Document to its PADInfo."@en .

pad:hasProvenance a owl:FunctionalProperty ;
    rdfs:domain pad:PAD ;
    rdfs:range pad:Provenance ;
    rdfs:label "has Provenance"@en ;
    rdfs:comment "The property relating a Platform Assertion Document to the Provenance of the Assertion."@en .

pad:hasSourceAssertion a owl:FunctionalProperty ;
    rdfs:domain pad:Assertion ;
    rdfs:range pad:Assertion ;
    rdfs:label "has Source Assertion"@en ;
    rdfs:comment "The property relating a Platform Assertion to a source Assertion where its data originated."@en .

pad:hasSourcePad a owl:FunctionalProperty ;
    rdfs:domain pad:PAD ;
    rdfs:range pad:PAD ;
    rdfs:label "has Source PAD"@en ;
    rdfs:comment "The property relating a Platform Assertion Document to a source Platform Assertion Document where its data originated."@en .

pad:hasProvenance a owl:FunctionalProperty ;
    rdfs:domain pad:PAD ;
    rdfs:range xsd:IRI ;
    rdfs:label "source Code"@en ;
    rdfs:comment "The property relating a Platform Assertion Document to the source code by which it was generated."@en .

dcterms:license a rdf:Property ;
    rdfs:domain rdfg:Graph ;
    rdfs:range xsd:IRI ;
    rdfs:label "License"@en ;
    rdfs:isDefinedBy <http://purl.org/dc/elements/1.1/license> .

dcterms:created a rdf:Property ;
    rdfs:domain rdfg:Graph ;
    rdfs:range xsd:DateTime ;
    rdfs:label "Created On"@en ;
    rdfs:isDefinedBy <http://purl.org/dc/elements/1.1/created> .

dcterms:creator a rdf:Property ;
    rdfs:domain rdfg:Graph ;
    rdfs:range dcterms:Agent ;
    rdfs:label "Creator"@en ;
    rdfs:isDefinedBy <http://purl.org/dc/elements/1.1/creator> .
