@prefix rdfg: <http://www.w3.org/2004/03/trix/rdfg-1/> .
@prefix rdfs: <http://www.w3.org/2000/01/rdf-schema#> .
@prefix rdf: <http://www.w3.org/1999/02/22-rdf-syntax-ns#> .
@prefix xsd: <http://www.w3.org/2001/XMLSchema#> .
@prefix owl: <http://www.w3.org/2002/07/owl#> .
@prefix doaj: <https://doaj.org/> .
@prefix dc: <http://purl.org/dc/elements/1.1/> .
@prefix dcterms: <http://purl.org/dc/terms/> .
@prefix fabio: <http://purl.org/spar/fabio/> .
@prefix foaf: <http://xmlns.com/foaf/0.1/> .
@prefix ppo: <http://purl.org/cwts/ppo/> .
@prefix pro: <http://purl.org/spar/pro/> .
@prefix pso: <http://purl.org/spar/pso/> .
@prefix loc: <http://id.loc.gov/ontologies/bibframe/> .
@prefix openalex: <https://openalex.org/> .
@prefix prism: <http://prismstandard.org/namespaces/basic/2.0/> .
@prefix romeo: <https://v2.sherpa.ac.uk/id/> .
@prefix schema: <https://schema.org/> .
@prefix wd: <http://www.wikidata.org/entity/> .
@prefix xsd: <http://www.w3.org/2001/XMLSchema#> .

ppo:ArticleProcessingCharges a owl:Class ;
    rdfs:label "Article Processing Charges"@en ;
    rdfs:comment "Article processing charges (APCs) are publication fees charged to authors of works during the publication process."@en .

ppo:EvaluationPolicy rdfs:subClassOf ppo:Policy ;
    rdfs:label "Evaluation Policy"@en ;
    rdfs:comment "A collection of rules and allowances that a platform maintains during the evaluation of a work."@en .

ppo:OptIn a owl:Class ;
    rdfs:label "Opt-In"@en ;
    rdfs:comment "A piece of information is made publicly available with the permission of all objects having a ppo:optInBy relation with this entity."@en .

ppo:Platform a owl:Class ;
    rdfs:label "Platform"@en ;
    rdfs:comment "A scholarly communication platform that plays some role in the publishing process (e.g. publication, hosting, reviewing, etc.)."@en .

ppo:PlatformType a owl:Class ;
    rdfs:label "Platform Type"@en ;
    rdfs:comment "The role that a platform can fulfill during the publication process."@en .

ppo:Policy a owl:Class ;
    rdfs:label "Policy"@en ;
    rdfs:comment "A collection of rules and allowances that a platform maintains."@en .

ppo:PublicAccessibility a owl:Class ;
    rdfs:label "Public Accessibility"@en ;
    rdfs:comment "Object that describes the public accessibility of an entity."@en .

ppo:PublicationElsewherePolicy rdfs:subClassOf ppo:Policy ;
    rdfs:label "Publication Elsewhere Policy"@en ;
    rdfs:comment "A collection of rules and allowances that a platform maintains regarding publication of works on other platforms."@en .

ppo:PublicationElsewhereAllowedPolicy rdfs:subClassOf ppo:PublicationElsewherePolicy ;
    rdfs:label "Publication Elsewhere Allowed Policy"@en ;
    rdfs:comment "A collection of rules and allowances that a platform maintains regarding allowing publication of works on other platforms."@en .

ppo:PublicationElsewhereProhibitedPolicy rdfs:subClassOf ppo:PublicationElsewherePolicy ;
    rdfs:label "Publication Elsewhere Prohibited Policy"@en ;
    rdfs:comment "A collection of rules and allowances that a platform maintains regarding prohibition of publication of works on other platforms."@en .

ppo:PublicationElsewhereMandatoryPolicy rdfs:subClassOf ppo:PublicationElsewherePolicy ;
    rdfs:label "Publication Elsewhere Mandatory Policy"@en ;
    rdfs:comment "A collection of rules and allowances that a platform maintains regarding mandating of publication of works on other platforms."@en .

ppo:PublicationPolicy rdfs:subClassOf ppo:Policy ;
    rdfs:label "Publication Policy"@en ;
    rdfs:comment "A collection of rules and allowances that a platform maintains during the publication of a work."@en .

ppo:Work a owl:Class ;
    rdfs:label "Work"@en ;
    rdfs:comment "A collection of rules and allowances that a platform maintains during the publication of a work."@en .

ppo:appliesToVersion a rdf:Property ;
    rdfs:domain pro:Policy ;
    rdfs:range pso:PublicationStatus ;
    rdfs:label "applies to Version"@en ;
    rdfs:comment "The version of the work to which the policy applies."@en .

ppo:anonymousTo a rdf:Property ;
    rdfs:domain pro:PublishingRole ;
    rdfs:range pro:PublishingRole ;
    rdfs:label "Anonymous To"@en ;
    rdfs:comment "The relation that signifies that the subject is not aware of the identity of the object."@en .

ppo:covers a rdf:Property ;
    rdfs:domain ppo:EvaluationPolicy ;
    rdfs:range ppo:DocumentType ;
    rdfs:label "covers"@en ;
    rdfs:comment "Relation that signifies that a policy includes restrictions or allowances on a particular type of document related to the work or policy."@en .

ppo:hasCrossrefId a rdf:Property ;
    rdfs:subPropertyOf dcterms:identifier ;
    rdfs:domain ppo:Platform ;
    rdfs:range xsd:anyURI ;
    rdfs:label "Crossref Identifier"@en ;
    rdfs:comment "Relation linking a platform to its Crossref identifier."@en .

ppo:hasDimensionsId a rdf:Property ;
    rdfs:subPropertyOf dcterms:identifier ;
    rdfs:domain ppo:Platform ;
    rdfs:range xsd:anyURI ;
    rdfs:label "Dimensions Identifier"@en ;
    rdfs:comment "Relation linking a platform to its Dimensions identifier."@en .

ppo:hasScopusId a rdf:Property ;
    rdfs:subPropertyOf dcterms:identifier ;
    rdfs:domain ppo:Platform ;
    rdfs:range xsd:anyURI ;
    rdfs:label "Scopus Identifier"@en ;
    rdfs:comment "Relation linking a platform to its Scopus identifier."@en .

ppo:hasMagId a rdf:Property ;
    rdfs:subPropertyOf dcterms:identifier ;
    rdfs:domain ppo:Platform ;
    rdfs:range xsd:anyURI ;
    rdfs:label "Microsoft Academic Graph Identifier"@en ;
    rdfs:comment "Relation linking a platform to its Microsoft Academic Graph identifier."@en .

ppo:hasArticleProcessingCharges a rdf:Property ;
    rdfs:domain ppo:PublicationPolicy ;
    rdfs:range ppo:ArticleProcessingCharges ;
    rdfs:label "has Article Processing Charges"@en ;
    rdfs:comment "A relation linking publication policies to article processing charges."@en .

ppo:hasCopyrightOwner a rdf:Property ;
    rdfs:domain ppo:Policy ;
    rdfs:range pro:PublishingRole ;
    rdfs:label "has Copyright Owner"@en ;
    rdfs:comment "Relation that signifies who retains the copyright over a work when published under the policy."@en .

ppo:hasFatcatId a rdf:Property ;
    rdfs:subPropertyOf dcterms:identifier ;
    rdfs:domain ppo:Platform ;
    rdfs:range xsd:anyURI ;
    rdfs:label "Fatcat Identifier"@en ;
    rdfs:comment "Relation linking a platform to its FatCat identifier."@en .

ppo:hasInitiator rdfs:subPropertyOf ppo:involves ;
    rdfs:domain ppo:EvaluationPolicy ;
    rdfs:range pro:PublishingRole ;
    rdfs:label "has Initiator"@en ;
    rdfs:comment "Relation that describes an agent as the initiator for a specific evaluation policy."@en .

ppo:hasOpenalexId a rdf:Property ;
    rdfs:subPropertyOf dcterms:identifier ;
    rdfs:domain ppo:Platform ;
    rdfs:range xsd:anyURI ;
    rdfs:label "OpenAlex Identifier"@en ;
    rdfs:comment "Relation linking a platform to its OpenAlex identifier."@en .

ppo:isOpenAccess a rdf:Property ;
    rdfs:domain ppo:PublicationPolicy ;
    rdfs:range xsd:boolean ;
    rdfs:label "is Open Access"@en ;
    rdfs:comment "Relation that signifies whether a work that the publication policy covers may be open access or not."@en .

ppo:hasPlatformType a rdf:Property ;
    rdfs:domain ppo:Platform ;
    rdfs:range xsd:string ;
    rdfs:label "has Platform Type"@en ;
    rdfs:comment "Relation linking a platform to a platform type."@en .

ppo:hasPolicy a rdf:Property ;
    rdfs:domain ppo:Platform, ppo:PlatformType ;
    rdfs:range ppo:Policy ;
    rdfs:label "has Policy"@en ;
    rdfs:comment "Relation linking a platform to a policy."@en .

ppo:hasSherpaRomeoId a rdf:Property ;
    rdfs:subPropertyOf dcterms:identifier ;
    rdfs:domain ppo:Platform ;
    rdfs:range xsd:anyURI ;
    rdfs:label "Sherpa-Romeo Identifier"@en ;
    rdfs:comment "Relation linking a platform to its Sherpa Romeo identifier."@en .

ppo:identityPubliclyAccessible a rdf:Property ;
    rdfs:domain pro:PublishingRole ;
    rdfs:range ppo:PublicAccessibility ;
    rdfs:subPropertyOf ppo:publiclyAccessible ;
    rdfs:label "identity Publicly Accessible"@en ;
    rdfs:comment "Relation that signifies the public availability of the identity of an agent."@en .

ppo:interactsWith a owl:SymmetricProperty ;
    rdfs:domain pro:PublishingRole ;
    rdfs:range pro:PublishingRole ;
    rdfs:label "interacts With"@en ;
    rdfs:comment "Relation that signifies that an agent can interact with another agent during the review process."@en .

ppo:involves a rdf:Property ;
    rdfs:domain ppo:Policy ;
    rdfs:range pro:PublishingRole ;
    rdfs:label "involves"@en ;
    rdfs:comment "Relation that signifies that an agent is involved during the process for a specific policy."@en .

ppo:optInBy a rdf:Property ;
    rdfs:domain ppo:OptIn ;
    rdfs:range pro:PublishingRole ;
    rdfs:label "opt-In By"@en ;
    rdfs:comment "Relation that signifies the permission of an agent for a specific thing to be made publicly accessible."@en .

ppo:postPublicationCommenting rdfs:subClassOf ppo:Work ;
    rdfs:isDefinedBy <https://osf.io/7j6ck> ;
    rdfs:label "Post Publication Commenting"@en ;
    rdfs:comment "Allowance of comments on the online published version of the version of record."@en .

ppo:publicationCondition a rdf:Property ;
    rdfs:domain ppo:PublicationElsewhereAllowedPolicy ;
    rdfs:range xsd:string ;
    rdfs:label "Publication Condition"@en ;
    rdfs:comment "Relation describing a condition for publication of a work on other platforms."@en .

ppo:publicationLocation a rdf:Property ;
    rdfs:domain ppo:PublicationElsewhereAllowedPolicy ;
    rdfs:range xsd:string ;
    rdfs:label "Publication Location"@en ;
    rdfs:comment "Relation describing a location condition for publication of a work on other platforms."@en .

ppo:publiclyAccessible a rdf:Property ;
    rdfs:domain ppo:Work ;
    rdfs:range ppo:PublicAccessibility ;
    rdfs:label "publicly Accessible"@en ;
    rdfs:comment "Relation that signifies the public availability of a work."@en .

ppo:Accessible a ppo:PublicAccessibility; a owl:NamedIndividual ;
    rdfs:label "Accessible"@en ;
    rdfs:comment "A piece of information is made publicly available."@en .

ppo:AuthorEditorCommunication a ppo:Work ; a owl:NamedIndividual ;
    rdfs:isDefinedBy <https://osf.io/7j6ck> ;
    rdfs:label "Author-Editor Communication"@en ;
    rdfs:comment "Communication between the author and editor of a work, including editor decision letter and reviewer responses (rebuttals)."@en .

ppo:NotAccessible a ppo:PublicAccessibility; a owl:NamedIndividual ;
    rdfs:label "Not Accessible"@en ;
    rdfs:comment "A piece of information is not made publicly available."@en .

ppo:postPublicationCommentingOpen a ppo:postPublicationCommenting; a owl:NamedIndividual ;
    rdfs:isDefinedBy <https://osf.io/7j6ck> ;
    rdfs:label "Post Publication Commenting Open"@en ;
    rdfs:comment "Post publication commenting is open."@en .

ppo:postPublicationCommentingClosed a ppo:postPublicationCommenting; a owl:NamedIndividual ;
    rdfs:isDefinedBy <https://osf.io/7j6ck> ;
    rdfs:label "Post Publication Commenting Closed"@en ;
    rdfs:comment "Post publication commenting is closed."@en .

ppo:postPublicationCommentingOnInvitation a ppo:postPublicationCommenting; a owl:NamedIndividual ;
    rdfs:isDefinedBy <https://osf.io/7j6ck> ;
    rdfs:label "Post Publication Commenting On Invitation"@en ;
    rdfs:comment "Post publication commenting is open on invitation only."@en .

ppo:ReviewReport a ppo:Work; a owl:NamedIndividual ;
    rdfs:isDefinedBy <https://osf.io/7j6ck> ;
    rdfs:label "Review Report"@en ;
    rdfs:comment "Full content of the peer review of a work by a peer-reviewer."@en .

ppo:ReviewSummary a ppo:Work; a owl:NamedIndividual ;
    rdfs:isDefinedBy <https://osf.io/7j6ck> ;
    rdfs:label "Review Summary"@en ;
    rdfs:comment "Summarized content of the peer review of a work by a peer-reviewer."@en .

pro:Society a foaf:Organization ;
    rdfs:isDefinedBy <http://purl.org/spar/pro/publisher> ;
    rdfs:label "Society"@en ;
    rdfs:comment "An organization that exists to promote an academic discipline, profession, or a group of related disciplines."@en .

ppo:SubmittedManuscript a ppo:Work; a owl:NamedIndividual ;
    rdfs:isDefinedBy <https://osf.io/7j6ck> ;
    rdfs:label "Submitted Manuscript"@en ;
    rdfs:comment "The version of the work submitted for peer-review."@en .

dcterms:LicenseDocument a owl:Class ;
    rdfs:label "License"@en ;
    rdfs:comment "A legal document giving official permission to do something with the resource."@en .

foaf:Organization a owl:Class ;
    rdfs:isDefinedBy <http://xmlns.com/foaf/0.1/Organization> ;
    rdfs:label "Organization"@en .

pro:PublishingRole a owl:Class ;
    rdfs:isDefinedBy <http://purl.org/spar/pro/PublishingRole> ;
    rdfs:label "Publishing Role"@en .

pso:PublicationStatus a rdf:Class ;
    rdfs:label "Publication Status"@en ;
    rdfs:comment "A state or condition that a work may have that relates to the publication of such work."@en .

dcterms:identifier a rdf:Property ;
    rdfs:domain ppo:Platform ;
    rdfs:range xsd:literal ;
    rdfs:isDefinedBy <http://purl.org/dc/elements/1.1/identifier> ;
    rdfs:label "Identifier"@en .

dcterms:license a rdf:Property ;
    rdfs:domain ppo:Assertion ;
    rdfs:range dcterms:LicenseDocument ;
    rdfs:isDefinedBy <http://purl.org/dc/elements/1.1/license> ;
    rdfs:label "License"@en .

dcterms:publisher a rdf:Property ;
    rdfs:subPropertyOf dcterms:relation ;
    rdfs:domain ppo:Platform ;
    rdfs:range foaf:Organization ;
    rdfs:isDefinedBy <http://purl.org/dc/elements/1.1/publisher> ;
    rdfs:label "has Publisher"@en .

dcterms:relation a rdf:Property ;
    rdfs:domain ppo:Platform ;
    rdfs:range foaf:Organization ;
    rdfs:isDefinedBy <http://purl.org/dc/elements/1.1/relation> ;
    rdfs:label "has Relation"@en .

fabio:hasEmbargoDuration a rdf:Property ;
    rdfs:domain ppo:PublicationPolicy ;
    rdfs:range xsd:duration ;
    rdfs:label "has Embargo Duration"@en ;
    rdfs:comment "The time period for which an work is embargoed. During this period, the work should not be published or, in the case of a press release, should not be reported on. For open-access journal articles, the embargo duration specifies that period of time during which availability of the open-access version of the work is delayed by the publisher, following subscription-access availability of the published work."@en .

fabio:hasIssnL a rdf:Property ;
    rdfs:subPropertyOf dcterms:identifier ;
    rdfs:domain ppo:Platform ;
    rdfs:range xsd:string ;
    rdfs:label "Linking ISSN"@en ;
    rdfs:comment "Linking International Standard Serial Number"@en .

prism:doi a rdf:Property ;
    rdfs:subPropertyOf dcterms:identifier ;
    rdfs:domain ppo:Platform ;
    rdfs:range xsd:string ;
    rdfs:label "DOI"@en ;
    rdfs:comment "Digital Object Identifier"@en .

prism:eIssn a rdf:Property ;
    rdfs:subPropertyOf dcterms:identifier ;
    rdfs:domain ppo:Platform ;
    rdfs:range xsd:string ;
    rdfs:label "Electronic ISSN"@en ;
    rdfs:comment "Electronic International Standard Serial Number"@en .

prism:issn a rdf:Property ;
    rdfs:subPropertyOf dcterms:identifier ;
    rdfs:domain ppo:Platform ;
    rdfs:range xsd:string ;
    rdfs:label "Print ISSN"@en ;
    rdfs:comment "Print International Standard Serial Number"@en .

schema:name a rdf:Property ;
    rdfs:range xsd:string ;
    rdfs:isDefinedBy <http://schema.org/name> ;
    rdfs:label "Name"@en .

schema:price a rdf:Property ;
    rdfs:range xsd:double ;
    rdfs:isDefinedBy <http://schema.org/price> ;
    rdfs:label "Price"@en .

schema:priceCurrency a rdf:Property ;
    rdfs:range xsd:string ;
    rdfs:isDefinedBy <http://schema.org/priceCurrency> ;
    rdfs:label "Currency"@en .

schema:url a rdf:Property ;
    rdfs:range xsd:anyURI ;
    rdfs:isDefinedBy <http://schema.org/url> ;
    rdfs:label "URL"@en .

wd:id a rdf:Property ;
    rdfs:subPropertyOf dcterms:identifier ;
    rdfs:domain ppo:Platform ;
    rdfs:range xsd:string ;
    rdfs:label "Wikidata Identifier"@en .

pro:author a pro:PublishingRole ;
    rdfs:isDefinedBy <http://purl.org/spar/pro/author> ;
    rdfs:label "Author"@en .

pro:editor a pro:PublishingRole ;
    rdfs:isDefinedBy <http://purl.org/spar/pro/editor> ;
    rdfs:label "Editor"@en .

pro:peer-reviewer a pro:PublishingRole ;
    rdfs:isDefinedBy <http://purl.org/spar/pro/peer-reviewer> ;
    rdfs:label "Peer Reviewer"@en .

pro:publisher a pro:PublishingRole ; a foaf:Organization ;
    rdfs:isDefinedBy <http://purl.org/spar/pro/publisher> ;
    rdfs:label "Publisher"@en .

pso:accepted-for-publication a pso:PublicationStatus ;
    rdfs:label "Accepted version"@en ;
    rdfs:comment "The status of a work (for example a document or a dataset) once it has been accepted for publication by a publisher or data repository."@en .

pso:published a pso:PublicationStatus ;
    rdfs:label "Published version"@en ;
    rdfs:comment "The status of a work (for example a document or a dataset) that has been published, i.e. made available for people to access, read or use, either freely or for a purchase price or an access fee."@en .

pso:submitted a pso:PublicationStatus ;
    rdfs:label "Submitted version"@en ;
    rdfs:comment "The status of a work (for example a document or a dataset) that has been submitted for publication by the author to a publisher or a data repository, prior to its being accepted or rejected."@en .

<https://creativecommons.org/publicdomain/zero/1.0> a dcterms:licenseDocument ;
    owl:sameAs <https://creativecommons.org/publicdomain/zero/1.0/> ;
    rdfs:label "CC0"@en .
<https://creativecommons.org/licenses/by/4.0> a dcterms:licenseDocument ;
    owl:sameAs <https://creativecommons.org/licenses/by/4.0/> ;
    rdfs:label "CC BY"@en .
<https://creativecommons.org/licenses/by-nc/4.0> a dcterms:licenseDocument ;
    owl:sameAs <https://creativecommons.org/licenses/by-nc/4.0/> ;
    rdfs:label "CC BY-NC"@en .
<https://creativecommons.org/licenses/by-nc-nd/4.0> a dcterms:licenseDocument ;
    owl:sameAs <https://creativecommons.org/licenses/by-nc-nd/4.0/> ;
    rdfs:label "CC BY-NC-ND"@en .
<https://creativecommons.org/licenses/by-nc-sa/4.0> a dcterms:licenseDocument ;
    owl:sameAs <https://creativecommons.org/licenses/by-nc-sa/4.0/> ;
    rdfs:label "CC BY-NC-SA"@en .
<https://creativecommons.org/licenses/by-nd/4.0> a dcterms:licenseDocument ;
    owl:sameAs <https://creativecommons.org/licenses/by-nd/4.0/> ;
    rdfs:label "CC BY-ND"@en .
<https://creativecommons.org/licenses/by-sa/4.0> a dcterms:licenseDocument ;
    owl:sameAs <https://creativecommons.org/licenses/by-sa/4.0/> ;
    rdfs:label "CC BY-SA"@en .
