@prefix rdfg: <http://www.w3.org/2004/03/trix/rdfg-1/> .
@prefix rdfs: <http://www.w3.org/2000/01/rdf-schema#> .
@prefix rdf: <http://www.w3.org/1999/02/22-rdf-syntax-ns#> .
@prefix xsd: <http://www.w3.org/2001/XMLSchema#> .
@prefix owl: <http://www.w3.org/2002/07/owl#> .
@prefix bibo: <http://purl.org/ontology/bibo/> .
@prefix doaj: <https://doaj.org/> .
@prefix dc: <http://purl.org/dc/elements/1.1/> .
@prefix dcterms: <http://purl.org/dc/terms/> .
@prefix fabio: <http://purl.org/spar/fabio/> .
@prefix foaf: <http://xmlns.com/foaf/0.1/> .
@prefix scpo: <http://purl.org/job/scpo/> .
@prefix pro: <http://purl.org/spar/pro/> .
@prefix pso: <http://purl.org/spar/pso/> .
@prefix loc: <http://id.loc.gov/ontologies/bibframe/> .
@prefix openalex: <https://openalex.org/> .
@prefix prism: <http://prismstandard.org/namespaces/basic/2.0/> .
@prefix romeo: <https://v2.sherpa.ac.uk/id/> .
@prefix schema: <https://schema.org/> .
@prefix wd: <http://www.wikidata.org/entity/> .
@prefix xsd: <http://www.w3.org/2001/XMLSchema#> .

scpo: a owl:Ontology ;
    dcterms:title "SCPO, the Scholarly Communication Platform Ontology" ;
    dcterms:creator "Bram van den Boomen" ;
    dcterms:creator "Nees Jan van Eck" ;
    dcterms:creator "Ludo Waltman" ;
    dcterms:creator "Serge Horbach" ;
    dcterms:creator "Tony Ross-Hellauer" ;
    dcterms:license <https://creativecommons.org/licenses/by/4.0/> ;
    dcterms:date "2023-04-21" ;
    bibo:status "Ontology Specification Draft" ;
    owl:versionInfo "0.1.0" ;
    foaf:image scpo:diagram.png ;
    dcterms:description """
The Scholarly Communication Platform Ontology (SCPO) models publication and evaluation policies of scholarly communication platforms.

Examples of properties describing platforms include:
- An identifier of a platform.
- A name of a platform.
- A URL of a platform.
- An organization managing a platform.
- A policy of a platform, for instance a publication policy (e.g., covering the organization of open access publishing) or an evaluation policy (e.g., covering the organization of peer review). In the next sections, we discuss how we model these policies.

A publication policy describes a policy of a scholarly communication platform for publishing research articles. Some platforms have multiple publication policies. For instance, a hybrid open access journal has a publication policy for closed access articles and a publication policy for open access articles. Other platforms, for instance peer review platforms, do not publish research articles and therefore do not have a publication policy.

In addition to publication policies, a scholarly communication platform may also have publication elsewhere policies. A publication elsewhere policy is a policy of a platform that prohibits, allows, or mandates the publication of a research article on other platforms. A platform may have different publication elsewhere policies for different versions of a research article.

The following examples illustrate the idea of a publication elsewhere policy:
- Some journals prohibit the publication of some or all versions of a research article on a preprint server (‘Ingelfinger rule’).
- Some journals allow the publication of some or all versions of a research article on a preprint server.
- Some journals mandate the publication of some or all versions of a research article on a preprint server. eLife is a well-known example. Overlay journals are another example.
- Peer review platforms typically mandate the publication of a research article in a journal or on a preprint server. It is not possible to publish a review of an article on these platforms if the article itself has not yet been published.

An evaluation policy describes the policy of a scholarly communication platform for evaluating research articles. Evaluation may range from in-depth peer review performed by many journals and peer review platforms to more superficial screening performed by many preprint servers. Some platforms, for instance repositories such as Zenodo, do not perform any evaluation and therefore do not have an evaluation policy. The approach taken in the SCPO to model evaluation policies builds on and extends the STM peer review terminology.

The evaluation of a research article may involve individuals with different roles, for instance authors, reviewers, and editors. These individuals may or may not know each others’ identity. In addition, the evaluation of an article may involve different types of documents. In addition to the article itself, the STM peer review terminology for instance distinguishes between review reports, review summaries, and author/editor communication.

Both the identities of the individuals involved in the evaluation of a research article and the documents involved in this may or may not be made public, or they may be made public only with the consent of specific individuals.
"""@en .

scpo:ArticleProcessingCharge a owl:Class ;
    rdfs:label "Article Processing Charge"@en ;
    rdfs:comment "The article processing charge (APC) that a platform charges to the authors of a scholarly work."@en .

scpo:EvaluationPolicy rdfs:subClassOf scpo:Policy ;
    rdfs:label "Evaluation Policy"@en ;
    rdfs:comment "A policy of a platform regarding the evaluation of a scholarly work."@en .

scpo:OptIn a owl:Class ;
    rdfs:label "Opt-In"@en ;
    rdfs:comment "A piece of information, such as a scholarly work or the identity of an agent, can be made publicly accessible only with the permissions of the relevant agents."@en .

scpo:Platform a owl:Class ;
    rdfs:label "Platform"@en ;
    rdfs:comment "A platform for scholarly communication, in particular for the publication and/or evaluation of scholarly works, such as a scientific journal, a preprint server or a peer review platform."@en .

scpo:PlatformType a owl:Class ;
    rdfs:label "Platform Type"@en ;
    rdfs:comment "A platform type, such as scientific journal, preprint server or peer review platform."@en .

scpo:Policy a owl:Class ;
    rdfs:label "Policy"@en ;
    rdfs:comment "A policy of a platform."@en .

scpo:PostPublicationCommenting rdfs:subClassOf scpo:Work ;
    rdfs:isDefinedBy <https://osf.io/7j6ck> ;
    rdfs:label "Post Publication Commenting"@en ;
    rdfs:comment "Allowance of post publication commenting on a scholarly work."@en .

scpo:PublicAccessibility a owl:Class ;
    rdfs:label "Public Accessibility"@en ;
    rdfs:comment "The public accessibility of a piece of information, such as a scholarly work or the identity of an agent."@en .

scpo:PublicationElsewherePolicy rdfs:subClassOf scpo:Policy ;
    rdfs:label "Publication Elsewhere Policy"@en ;
    rdfs:comment "A policy of a platform regarding the publication of a scholarly work on other platforms."@en .

scpo:PublicationElsewhereAllowedPolicy rdfs:subClassOf scpo:PublicationElsewherePolicy ;
    rdfs:label "Publication Elsewhere Allowed Policy"@en ;
    rdfs:comment "A policy of a platform that allows the publication of a scholarly work on other platforms."@en .

scpo:PublicationElsewhereProhibitedPolicy rdfs:subClassOf scpo:PublicationElsewherePolicy ;
    rdfs:label "Publication Elsewhere Prohibited Policy"@en ;
    rdfs:comment "A policy of a platform that prohibits the publication of a scholarly work on other platforms."@en .

scpo:PublicationElsewhereMandatoryPolicy rdfs:subClassOf scpo:PublicationElsewherePolicy ;
    rdfs:label "Publication Elsewhere Mandatory Policy"@en ;
    rdfs:comment "A policy of a platform that mandates the publication of a scholarly work on other platforms."@en .

scpo:PublicationPolicy rdfs:subClassOf scpo:Policy ;
    rdfs:label "Publication Policy"@en ;
    rdfs:comment "A policy of a platform regarding the publication of a scholarly work."@en .

scpo:Work a owl:Class ;
    rdfs:label "Work"@en ;
    rdfs:comment "A scholarly work, such as a research article, review report or review summary."@en .

scpo:appliesToVersion a rdf:Property ;
    rdfs:domain pro:Policy ;
    rdfs:range pso:PublicationStatus ;
    rdfs:label "applies to Version"@en ;
    rdfs:comment "Relation signifying the version of a scholarly work to which a policy applies."@en .

scpo:anonymousTo a rdf:Property ;
    rdfs:domain pro:PublishingRole ;
    rdfs:range pro:PublishingRole ;
    rdfs:label "Anonymous To"@en ;
    rdfs:comment "Relation signifying that an agent is not aware of the identity of another agent in an evaluation process."@en .

scpo:covers a rdf:Property ;
    rdfs:domain scpo:Policy ;
    rdfs:range scpo:Work ;
    rdfs:label "covers"@en ;
    rdfs:comment "Relation signifying that a policy includes restrictions or allowances on a scholarly work."@en .

scpo:hasCrossrefId a rdf:Property ;
    rdfs:subPropertyOf dcterms:identifier ;
    rdfs:domain scpo:Platform ;
    rdfs:range xsd:anyURI ;
    rdfs:label "Crossref Identifier"@en ;
    rdfs:comment "Relation linking a platform to its Crossref identifier."@en .

scpo:hasDimensionsId a rdf:Property ;
    rdfs:subPropertyOf dcterms:identifier ;
    rdfs:domain scpo:Platform ;
    rdfs:range xsd:anyURI ;
    rdfs:label "Dimensions Identifier"@en ;
    rdfs:comment "Relation linking a platform to its Dimensions identifier."@en .

scpo:hasScopusId a rdf:Property ;
    rdfs:subPropertyOf dcterms:identifier ;
    rdfs:domain scpo:Platform ;
    rdfs:range xsd:anyURI ;
    rdfs:label "Scopus Identifier"@en ;
    rdfs:comment "Relation linking a platform to its Scopus identifier."@en .

scpo:hasMagId a rdf:Property ;
    rdfs:subPropertyOf dcterms:identifier ;
    rdfs:domain scpo:Platform ;
    rdfs:range xsd:anyURI ;
    rdfs:label "Microsoft Academic Graph Identifier"@en ;
    rdfs:comment "Relation linking a platform to its Microsoft Academic Graph identifier."@en .

scpo:hasArticleProcessingCharge a rdf:Property ;
    rdfs:domain scpo:PublicationPolicy ;
    rdfs:range scpo:ArticleProcessingCharge ;
    rdfs:label "has Article Processing Charge"@en ;
    rdfs:comment "Relation linking a publication policy to an article processing charge."@en .

scpo:hasCopyrightOwner a rdf:Property ;
    rdfs:domain scpo:Policy ;
    rdfs:range pro:PublishingRole ;
    rdfs:label "has Copyright Owner"@en ;
    rdfs:comment "Relation linking a publication policy to a copyright owner."@en .

scpo:hasFatcatId a rdf:Property ;
    rdfs:subPropertyOf dcterms:identifier ;
    rdfs:domain scpo:Platform ;
    rdfs:range xsd:anyURI ;
    rdfs:label "Fatcat Identifier"@en ;
    rdfs:comment "Relation linking a platform to its FatCat identifier."@en .

scpo:hasInitiator rdfs:subPropertyOf scpo:involves ;
    rdfs:domain scpo:EvaluationPolicy ;
    rdfs:range pro:PublishingRole ;
    rdfs:label "has Initiator"@en ;
    rdfs:comment "Relation linking an evaluation policy to the agent that initiates an evaluation."@en .

scpo:hasOpenalexId a rdf:Property ;
    rdfs:subPropertyOf dcterms:identifier ;
    rdfs:domain scpo:Platform ;
    rdfs:range xsd:anyURI ;
    rdfs:label "OpenAlex Identifier"@en ;
    rdfs:comment "Relation linking a platform to its OpenAlex identifier."@en .

scpo:isOpenAccess a rdf:Property ;
    rdfs:domain scpo:PublicationPolicy ;
    rdfs:range xsd:boolean ;
    rdfs:label "is Open Access"@en ;
    rdfs:comment "Relation signifying whether a publication policy suscports open access publishing."@en .

scpo:hasPlatformType a rdf:Property ;
    rdfs:domain scpo:Platform ;
    rdfs:range xsd:PlatformType ;
    rdfs:label "has Platform Type"@en ;
    rdfs:comment "Relation linking a platform to a platform type."@en .

scpo:hasPolicy a rdf:Property ;
    rdfs:domain scpo:Platform, scpo:PlatformType ;
    rdfs:range scpo:Policy ;
    rdfs:label "has Policy"@en ;
    rdfs:comment "Relation linking a platform to a policy."@en .

scpo:hasPostPublicationCommenting a rdf:Property ;
    rdfs:domain scpo:EvaluationPolicy ;
    rdfs:range scpo:PostPublicationCommenting ;
    rdfs:label "Has Post Publication Commenting"@en ;
    rdfs:comment "Relation signifying whether an evaluation policy allows post publication commenting."@en .

scpo:hasSherpaRomeoId a rdf:Property ;
    rdfs:subPropertyOf dcterms:identifier ;
    rdfs:domain scpo:Platform ;
    rdfs:range xsd:anyURI ;
    rdfs:label "Sherpa-Romeo Identifier"@en ;
    rdfs:comment "Relation linking a platform to its Sherpa Romeo identifier."@en .

scpo:identityPubliclyAccessible a rdf:Property ;
    rdfs:domain pro:PublishingRole ;
    rdfs:range scpo:PublicAccessibility ;
    rdfs:subPropertyOf scpo:publiclyAccessible ;
    rdfs:label "identity Publicly Accessible"@en ;
    rdfs:comment "Relation signifying the public accessibility of the identity of an agent."@en .

scpo:interactsWith a owl:SymmetricProperty ;
    rdfs:domain pro:PublishingRole ;
    rdfs:range pro:PublishingRole ;
    rdfs:label "interacts With"@en ;
    rdfs:comment "Relation that signifies that an agent can interact with another agent during the review process."@en .

scpo:involves a rdf:Property ;
    rdfs:domain scpo:Policy ;
    rdfs:range pro:PublishingRole ;
    rdfs:label "involves"@en ;
    rdfs:comment "Relation signifying that a policy involves an agent."@en .

scpo:optInBy a rdf:Property ;
    rdfs:domain scpo:OptIn ;
    rdfs:range pro:PublishingRole ;
    rdfs:label "opt-In By"@en ;
    rdfs:comment "Relation signifying the permission of an agent to make a piece of information, such as a scholarly work or the identity of an agent, publicly accessible."@en .

scpo:publicationCondition a rdf:Property ;
    rdfs:domain scpo:PublicationElsewhereAllowedPolicy ;
    rdfs:range xsd:string ;
    rdfs:label "Publication Condition"@en ;
    rdfs:comment "Relation describing a condition for allowing publication of a scholarly work on other platforms."@en .

scpo:publicationLocation a rdf:Property ;
    rdfs:domain scpo:PublicationElsewhereAllowedPolicy ;
    rdfs:range xsd:string ;
    rdfs:label "Publication Location"@en ;
    rdfs:comment "Relation describing a condition for allowing publication of a scholarly work on specific types of other platforms."@en .

scpo:publiclyAccessible a rdf:Property ;
    rdfs:range scpo:PublicAccessibility ;
    rdfs:label "publicly Accessible"@en ;
    rdfs:comment "Relation signifying the public accessibility of a piece of information."@en .

scpo:workPubliclyAccessible a rdf:Property ;
    rdfs:domain scpo:Work ;
    rdfs:range scpo:PublicAccessibility ;
    rdfs:subPropertyOf scpo:publiclyAccessible ;
    rdfs:label "Work Publicly Accessible"@en ;
    rdfs:comment "Relation signifying the public accessibility  of a scholarly work."@en .

scpo:Accessible a scpo:PublicAccessibility; a owl:NamedIndividual ;
    rdfs:label "Accessible"@en ;
    rdfs:comment "A piece of information, such as a scholarly work or the identity of an agent, can be made publicly accessible."@en .

scpo:AuthorEditorCommunication a scpo:Work ; a owl:NamedIndividual ;
    rdfs:isDefinedBy <https://osf.io/7j6ck> ;
    rdfs:label "Author-Editor Communication"@en ;
    rdfs:comment "Communication between the author and editor of a scholarly work, including editor decision letter and reviewer responses (rebuttals)."@en .

scpo:NotAccessible a scpo:PublicAccessibility; a owl:NamedIndividual ;
    rdfs:label "Not Accessible"@en ;
    rdfs:comment "A piece of information, such as a scholarly work or the identity of an agent, can not be made publicly accessible."@en .

scpo:postPublicationCommentingOpen a scpo:postPublicationCommenting; a owl:NamedIndividual ;
    rdfs:isDefinedBy <https://osf.io/7j6ck> ;
    rdfs:label "Post Publication Commenting Open"@en ;
    rdfs:comment "Post publication commenting is open."@en .

scpo:postPublicationCommentingClosed a scpo:postPublicationCommenting; a owl:NamedIndividual ;
    rdfs:isDefinedBy <https://osf.io/7j6ck> ;
    rdfs:label "Post Publication Commenting Closed"@en ;
    rdfs:comment "Post publication commenting is closed."@en .

scpo:postPublicationCommentingOnInvitation a scpo:postPublicationCommenting; a owl:NamedIndividual ;
    rdfs:isDefinedBy <https://osf.io/7j6ck> ;
    rdfs:label "Post Publication Commenting On Invitation"@en ;
    rdfs:comment "Post publication commenting is open on invitation only."@en .

scpo:ReviewReport a scpo:Work; a owl:NamedIndividual ;
    rdfs:isDefinedBy <https://osf.io/7j6ck> ;
    rdfs:label "Review Report"@en ;
    rdfs:comment "Full content of the peer review of a scholarly work."@en .

scpo:ReviewSummary a scpo:Work; a owl:NamedIndividual ;
    rdfs:isDefinedBy <https://osf.io/7j6ck> ;
    rdfs:comment "Summarized content of the peer review of a scholarly work by a peer reviewer."@en .

pro:Society a foaf:Organization ;
    rdfs:label "Society"@en ;
    rdfs:comment "A scholarly society."@en .

scpo:SubmittedManuscript a scpo:Work; a owl:NamedIndividual ;
    rdfs:isDefinedBy <https://osf.io/7j6ck> ;
    rdfs:label "Submitted Manuscript"@en ;
    rdfs:comment "A scholarly work submitted to a platform and not yet accepted or rejected for publication on the platform."@en .

dcterms:LicenseDocument a owl:Class ;
    rdfs:label "License"@en ;
    rdfs:comment "A legal document giving official permission to do something with the resource."@en .

foaf:Organization a owl:Class ;
    rdfs:isDefinedBy <http://xmlns.com/foaf/0.1/Organization> ;
    rdfs:label "Organization"@en .

pro:PublishingRole a owl:Class ;
    rdfs:isDefinedBy <http://purl.org/spar/pro/PublishingRole> ;
    rdfs:label "Publishing Role"@en .

pso:PublicationStatus a rdf:Class ;
    rdfs:label "Publication Status"@en ;
    rdfs:comment "A state or condition that a work may have that relates to the publication of such work."@en .

dcterms:identifier a rdf:Property ;
    rdfs:isDefinedBy <http://purl.org/dc/elements/1.1/identifier> ;
    rdfs:label "Identifier"@en .

dcterms:license a rdf:Property ;
    rdfs:isDefinedBy <http://purl.org/dc/elements/1.1/license> ;
    rdfs:label "License"@en .

dcterms:publisher a rdf:Property ;
    rdfs:subPropertyOf dcterms:relation ;
    rdfs:isDefinedBy <http://purl.org/dc/elements/1.1/publisher> ;
    rdfs:label "has Publisher"@en .

dcterms:relation a rdf:Property ;
    rdfs:isDefinedBy <http://purl.org/dc/elements/1.1/relation> ;
    rdfs:label "has Relation"@en .

fabio:hasEmbargoDuration a rdf:Property ;
    rdfs:label "has Embargo Duration"@en ;
    rdfs:comment "The duration of the period in which a scholarly work is under embargo (i.e., the work has been published on a platform but has not yet been made openly accessible)."@en .

fabio:hasIssnL a rdf:Property ;
    rdfs:subPropertyOf dcterms:identifier ;
    rdfs:label "Linking ISSN"@en ;
    rdfs:comment "Linking International Standard Serial Number (ISSN)"@en .

prism:doi a rdf:Property ;
    rdfs:subPropertyOf dcterms:identifier ;
    rdfs:label "DOI"@en ;
    rdfs:comment "Digital Object Identifier (DOI)"@en .

prism:eIssn a rdf:Property ;
    rdfs:subPropertyOf dcterms:identifier ;
    rdfs:label "Electronic ISSN"@en ;
    rdfs:comment "Electronic International Standard Serial Number (ISSN)"@en .

prism:issn a rdf:Property ;
    rdfs:subPropertyOf dcterms:identifier ;
    rdfs:label "Print ISSN"@en ;
    rdfs:comment "Print International Standard Serial Number (ISSN)"@en .

schema:name a rdf:Property ;
    rdfs:label "Name"@en .

schema:price a rdf:Property ;
    rdfs:label "Price"@en .

schema:priceCurrency a rdf:Property ;
    rdfs:label "Currency"@en .

schema:url a rdf:Property ;
    rdfs:label "URL"@en .

wd:id a rdf:Property ;
    rdfs:subPropertyOf dcterms:identifier ;
    rdfs:label "Wikidata Identifier"@en .

pro:author a pro:PublishingRole ;
    rdfs:label "Author"@en .

pro:editor a pro:PublishingRole ;
    rdfs:label "Editor"@en .

pro:peer-reviewer a pro:PublishingRole ;
    rdfs:label "Peer Reviewer"@en .

pro:publisher a pro:PublishingRole ; a foaf:Organization ;
    rdfs:label "Publisher"@en .

scpo:accepted-for-publication a pso:PublicationStatus ;
    rdfs:label "Accepted version"@en ;
    rdfs:comment "The status of a scholarly work that has been accepted for publication on a platform."@en .

pso:published a pso:PublicationStatus ;
    rdfs:label "Published version"@en ;
    rdfs:comment "The status of a scholarly work that has been published on a platform in its final form."@en .

pso:submitted a pso:PublicationStatus ;
    rdfs:label "Submitted version"@en ;
    rdfs:comment "The status of a scholarly work that has been submitted to a platform and that has not yet been accepted or rejected for publication on the platform."@en .

<https://creativecommons.org/publicdomain/zero/1.0> a dcterms:licenseDocument ;
    owl:sameAs <https://creativecommons.org/publicdomain/zero/1.0/> ;
    rdfs:label "CC0"@en .
<https://creativecommons.org/licenses/by/4.0> a dcterms:licenseDocument ;
    owl:sameAs <https://creativecommons.org/licenses/by/4.0/> ;
    rdfs:label "CC BY"@en .
<https://creativecommons.org/licenses/by-nc/4.0> a dcterms:licenseDocument ;
    owl:sameAs <https://creativecommons.org/licenses/by-nc/4.0/> ;
    rdfs:label "CC BY-NC"@en .
<https://creativecommons.org/licenses/by-nc-nd/4.0> a dcterms:licenseDocument ;
    owl:sameAs <https://creativecommons.org/licenses/by-nc-nd/4.0/> ;
    rdfs:label "CC BY-NC-ND"@en .
<https://creativecommons.org/licenses/by-nc-sa/4.0> a dcterms:licenseDocument ;
    owl:sameAs <https://creativecommons.org/licenses/by-nc-sa/4.0/> ;
    rdfs:label "CC BY-NC-SA"@en .
<https://creativecommons.org/licenses/by-nd/4.0> a dcterms:licenseDocument ;
    owl:sameAs <https://creativecommons.org/licenses/by-nd/4.0/> ;
    rdfs:label "CC BY-ND"@en .
<https://creativecommons.org/licenses/by-sa/4.0> a dcterms:licenseDocument ;
    owl:sameAs <https://creativecommons.org/licenses/by-sa/4.0/> ;
    rdfs:label "CC BY-SA"@en .
